James C - added remaining opcodes to stack (flattening still broken)

FlatStack/FlatStackLanguage.thy
@@ -4,12 +4,14 @@ begin
 
 datatype flat_stack_instruction = 
   FAdd | FSub | FNeg | FEq | FGt | FLt | FAnd | FOr | FNot
-| Dup nat | Upd nat
+| FCon int | FDup nat | FUpd nat
+| FIf "flat_stack_instruction list" "flat_stack_instruction list"
+| FGoto code_label\<^sub>2
 | FPrint
 
-type_synonym flat_stack_program = "code_label \<rightharpoonup> flat_stack_instruction list \<times> code_label"
+type_synonym flat_stack_program = "code_label\<^sub>2 \<rightharpoonup> flat_stack_instruction list \<times> code_label\<^sub>2"
 
-type_synonym flat_stack_state = "int list \<times> flat_stack_instruction list \<times> code_label \<times> output" 
+type_synonym flat_stack_state = "int list \<times> flat_stack_instruction list \<times> code_label\<^sub>2 \<times> output" 
   (* \<sigma>, \<pi>, s, \<omega> *)
 
 inductive eval_flat_stack :: "flat_stack_program \<Rightarrow> flat_stack_state \<Rightarrow> flat_stack_state \<Rightarrow> bool" where
@@ -26,10 +28,17 @@ inductive eval_flat_stack :: "flat_stack_program \<Rightarrow> flat_stack_state 
     (unboolify (boolify i1 \<or> boolify i2) # \<sigma>, \<pi>, s, \<omega>)"
 | evf_not [simp]: "eval_flat_stack \<Pi> (i1 # \<sigma>, FNot # \<pi>, s, \<omega>) 
     (unboolify (\<not> boolify i1) # \<sigma>, \<pi>, s, \<omega>)"
-| evf_dup [simp]: "n < length \<sigma> \<Longrightarrow> eval_flat_stack \<Pi> (\<sigma>, Dup n # \<pi>, s, \<omega>) 
-    (\<sigma> ! n # \<sigma>, \<pi>, s, \<omega>)"
-| evf_upd [simp]: "n < length \<sigma> \<Longrightarrow> eval_flat_stack \<Pi> (i1 # \<sigma>, Upd n # \<pi>, s, \<omega>) 
-    (\<sigma>[n := i1], \<pi>, s, \<omega>)"
+| evf_con [simp]: "eval_flat_stack \<Pi> (\<sigma>, FCon i1 # \<pi>, s, \<omega>) (i1 # \<sigma>, \<pi>, s, \<omega>)"
+| evf_dup [simp]: "n < length \<sigma> \<Longrightarrow> 
+    eval_flat_stack \<Pi> (\<sigma>, FDup n # \<pi>, s, \<omega>) (\<sigma> ! n # \<sigma>, \<pi>, s, \<omega>)"
+| evf_upd [simp]: "n < length \<sigma> \<Longrightarrow> 
+    eval_flat_stack \<Pi> (i1 # \<sigma>, FUpd n # \<pi>, s, \<omega>) (\<sigma>[n := i1], \<pi>, s, \<omega>)"
+| evs_if_t [simp]: "boolify i1 \<Longrightarrow> 
+    eval_flat_stack \<Pi> (i1 # \<sigma>, FIf \<pi>\<^sub>t \<pi>\<^sub>f # \<pi>, s, \<omega>) (\<sigma>, \<pi>\<^sub>t @ \<pi>, s, \<omega>)"
+| evs_if_f [simp]: "\<not> boolify i1 \<Longrightarrow> 
+    eval_flat_stack \<Pi> (i1 # \<sigma>, FIf \<pi>\<^sub>t \<pi>\<^sub>f # \<pi>, s, \<omega>) (\<sigma>, \<pi>\<^sub>f @ \<pi>, s, \<omega>)"
+| evs_goto [simp]: "\<Pi> s = Some (\<pi>', s') \<Longrightarrow> 
+    eval_flat_stack \<Pi> (\<sigma>, FGoto s # \<pi>, s'', \<omega>) (\<sigma>, \<pi>', s', \<omega>)"
 | evf_print [simp]: "eval_flat_stack \<Pi> (i1 # \<sigma>, FPrint # \<pi>, s, \<omega>) (\<sigma>, \<pi>, s, i1 # \<omega>)"
 
 fun flat_stack_output :: "flat_stack_state \<Rightarrow> output" where
