Stack/Flattening.thy
@@ -2,44 +2,66 @@ theory Flattening
 imports StackLanguage "../FlatStack/FlatStackLanguage" "../Utilities/Iterate"
 begin
 
-fun instruction_convert :: "stack_instruction \<Rightarrow> flat_stack_instruction" where
-  "instruction_convert Add = FAdd"
-| "instruction_convert Sub = FSub"
-| "instruction_convert Neg = FNeg"
-| "instruction_convert Eq = FEq"
-| "instruction_convert Gt = FGt"
-| "instruction_convert Lt = FLt"
-| "instruction_convert And = FAnd"
-| "instruction_convert Or = FOr"
-| "instruction_convert Not = FNot"
-| "instruction_convert (Push (Constant i)) = undefined"
-| "instruction_convert (Push (Local v)) = undefined"
-| "instruction_convert (Push (Argument v)) = undefined"
-| "instruction_convert (Pop (Constant i)) = undefined"
-| "instruction_convert (Pop (Local v)) = undefined"
-| "instruction_convert (Pop (Argument v)) = undefined"
-| "instruction_convert Print = FPrint"
+fun instruction_convert :: "function_name \<Rightarrow> nat \<Rightarrow> nat \<Rightarrow> stack_instruction list \<Rightarrow> 
+    flat_stack_instruction list" where
+  "instruction_convert f ss ls [] = []"
+| "instruction_convert f ss ls (Add # \<pi>) = FAdd # instruction_convert f (ss - 1) ls \<pi>"
+| "instruction_convert f ss ls (Sub # \<pi>) = FSub # instruction_convert f (ss - 1) ls \<pi>"
+| "instruction_convert f ss ls (Neg # \<pi>) = FNeg # instruction_convert f ss ls \<pi>"
+| "instruction_convert f ss ls (Eq # \<pi>) = FEq # instruction_convert f (ss - 1) ls \<pi>"
+| "instruction_convert f ss ls (Gt # \<pi>) = FGt # instruction_convert f (ss - 1) ls \<pi>"
+| "instruction_convert f ss ls (Lt # \<pi>) = FLt # instruction_convert f (ss - 1) ls \<pi>"
+| "instruction_convert f ss ls (And # \<pi>) = FAnd # instruction_convert f (ss - 1) ls \<pi>"
+| "instruction_convert f ss ls (Or # \<pi>) = FOr # instruction_convert f (ss - 1) ls \<pi>"
+| "instruction_convert f ss ls (Not # \<pi>) = FNot # instruction_convert f ss ls \<pi>"
+| "instruction_convert f ss ls (Push (Constant i) # \<pi>) = 
+    FCon i # instruction_convert f (Suc ss) ls \<pi>"
+| "instruction_convert f ss ls (Push (Local v) # \<pi>) = 
+    FDup (ss + v) # instruction_convert f (Suc ss) ls \<pi>"
+| "instruction_convert f ss ls (Push (Argument v) # \<pi>) = 
+    FDup (ss + ls + v) # instruction_convert f (Suc ss) ls \<pi>"
+| "instruction_convert f ss ls (Pop (Constant i) # \<pi>) = FUpd 0 # instruction_convert f (ss - 1) ls \<pi>"
+| "instruction_convert f ss ls (Pop (Local v) # \<pi>) = 
+    FUpd (ss + v) # instruction_convert f (ss - 1) ls \<pi>"
+| "instruction_convert f ss ls (Pop (Argument v) # \<pi>) = 
+    FUpd (ss + ls + v) # instruction_convert f (ss - 1) ls \<pi>"
+| "instruction_convert f ss ls (IfJ \<pi>\<^sub>t \<pi>\<^sub>f # \<pi>) = 
+    FIf (instruction_convert f (ss - 1) ls \<pi>\<^sub>t) (instruction_convert f (ss - 1) ls \<pi>\<^sub>f) # 
+      instruction_convert f 0 ls \<pi>"
+| "instruction_convert f ss ls (Goto s # \<pi>) = [FGoto (CL\<^sub>2 f s)]"
+| "instruction_convert f ss ls (Call f' # \<pi>) = undefined # instruction_convert f (ss - 1) ls \<pi>"
+| "instruction_convert f ss ls (Return # \<pi>) = undefined # []"
+| "instruction_convert f ss ls (Print # \<pi>) = FPrint # instruction_convert f (ss - 1) ls \<pi>"
 
 primrec stack_value_convert :: "stack_value \<Rightarrow> int" where
   "stack_value_convert (IntV i) = i"
 | "stack_value_convert (Bool b) = unboolify b"
 
-definition flatten :: "stack_program \<Rightarrow> flat_stack_program" where
-  "flatten \<Pi> = map_option (\<lambda>(\<pi>, s). (map instruction_convert \<pi>, s)) o \<Pi>"
+primrec flatten :: "stack_program \<Rightarrow> flat_stack_program" where
+  "flatten \<Pi> (CL\<^sub>2 f s) = (case \<Pi> f of 
+      Some (a, ls, \<Phi>) \<Rightarrow> (case \<Phi> s of
+          Some (\<pi>, s') \<Rightarrow> Some (instruction_convert f 0 ls \<pi>, CL\<^sub>2 f s')
+        | None \<Rightarrow> None)
+    | None \<Rightarrow> None)"
+
+primrec flatten_frame :: "frame \<Rightarrow> int list" where
+  "flatten_frame (Frame f as ls \<sigma>) = map stack_value_convert (as @ ls @ \<sigma>)"
 
 fun state_convert :: "stack_state \<Rightarrow> flat_stack_state" where
-  "state_convert (\<sigma>, \<phi>, \<pi>, s, \<omega>) = (map stack_value_convert \<sigma>, map instruction_convert \<pi>, s, \<omega>)"
+  "state_convert (\<sigma>, \<phi>, \<pi>, s, \<omega>) = (case hd \<phi> of
+      Frame f as ls \<sigma> \<Rightarrow> (map stack_value_convert \<sigma> @ concat (map flatten_frame \<phi>), 
+        instruction_convert f (length \<sigma>) (length ls) \<pi>, CL\<^sub>2 f s, \<omega>))"
 
 (* flattening correct *)
 
 lemma [simp]: "flat_stack_output (state_convert \<Sigma>\<^sub>S) = stack_output \<Sigma>\<^sub>S"
-  by (induction \<Sigma>\<^sub>S rule: state_convert.induct) simp
+  proof (induction \<Sigma>\<^sub>S rule: state_convert.induct) 
+  case (1 \<sigma> \<phi> \<pi> s \<omega>)
+    thus ?case by (cases "hd \<phi>") simp
+  qed
 
 lemma [simp]: "finite (dom \<Pi>) \<Longrightarrow> finite (dom (flatten \<Pi>))"
-  by (simp add: flatten_def)
-
-lemma [simp]: "\<Pi> s = Some (\<pi>, s') \<Longrightarrow> flatten \<Pi> s = Some (map instruction_convert \<pi>, s')"
-  by (simp add: flatten_def)
+  by simp
 
 lemma [simp]: "eval_flat_stack (flatten \<Pi>) (unboolify b1 # unboolify b2 # \<sigma>, FAnd # \<pi>, s, \<omega>) 
     (unboolify (b2 \<and> b1) # \<sigma>, \<pi>, s, \<omega>)"
@@ -55,7 +77,67 @@ lemma [simp]: "eval_flat_stack (flatten \<Pi>) (unboolify b # \<sigma>, FNot # \
 
 lemma [simp]: "eval_stack \<Pi> \<Sigma> \<Sigma>' \<Longrightarrow> 
     eval_flat_stack (flatten \<Pi>) (state_convert \<Sigma>) (state_convert \<Sigma>')"
-  by (induction \<Pi> \<Sigma> \<Sigma>' rule: eval_stack.induct) simp_all
+  proof (induction \<Pi> \<Sigma> \<Sigma>' rule: eval_stack.induct)
+  case evs_jump
+    thus ?case by simp
+  next case evs_add
+    thus ?case by simp
+  next case evs_sub
+    thus ?case by simp
+  next case evs_neg
+    thus ?case by simp
+  next case evs_eq
+    thus ?case by simp
+  next case evs_gt
+    thus ?case by simp
+  next case evs_lt
+    thus ?case by simp
+  next case evs_and
+    thus ?case by simp
+  next case evs_or
+    thus ?case by simp
+  next case evs_not
+    thus ?case by simp
+  next case evs_push_c
+    thus ?case by simp
+  next case evs_goto
+    thus ?case by simp
+  next case evs_print
+    thus ?case by simp
+  next case (evs_push_l \<Pi> \<sigma> as ls \<phi> n \<pi> s \<omega>)
+    
+
+    have "eval_flat_stack (flatten \<Pi>) (state_convert (\<sigma>, Frame as ls # \<phi>, Push (Local n) # \<pi>, s, \<omega>)) (state_convert (ls ! n # \<sigma>, \<phi>, \<pi>, s, \<omega>))" by simp
+    thus ?case by simp
+  next case (evs_push_a \<Pi> \<sigma> as ls \<phi> n \<pi> s \<omega>)
+
+    have "eval_flat_stack (flatten \<Pi>) (state_convert (\<sigma>, Frame as ls # \<phi>, Push (Argument n) # \<pi>, s, \<omega>)) (state_convert (as ! n # \<sigma>, \<phi>, \<pi>, s, \<omega>))" by simp
+    thus ?case by simp
+  next case (evs_pop_l \<Pi> i \<sigma> as ls \<phi> n \<pi> s \<omega>)
+
+    have "eval_flat_stack (flatten \<Pi>) (state_convert (i # \<sigma>, Frame as ls # \<phi>, Pop (Local n) # \<pi>, s, \<omega>)) (state_convert (\<sigma>, Frame as (ls[n := i]) # \<phi>, \<pi>, s, \<omega>))" by simp
+    thus ?case by simp
+  next case (evs_pop_a \<Pi> i \<sigma> as ls \<phi> n \<pi> s \<omega>) 
+
+    have "eval_flat_stack (flatten \<Pi>) (state_convert (i # \<sigma>, Frame as ls # \<phi>, Pop (Argument n) # \<pi>, s, \<omega>)) (state_convert (\<sigma>, Frame (as[n := i]) ls # \<phi>, \<pi>, s, \<omega>))" by simp
+    thus ?case by simp
+  next case (evs_if_t \<Pi> \<sigma> \<phi> \<pi>\<^sub>t \<pi>\<^sub>f \<pi> s \<omega>)
+
+    have "eval_flat_stack (flatten \<Pi>) (state_convert (Bool True # \<sigma>, \<phi>, IfJ \<pi>\<^sub>t \<pi>\<^sub>f # \<pi>, s, \<omega>)) (state_convert (\<sigma>, \<phi>, \<pi>\<^sub>t @ \<pi>, s, \<omega>))" by simp
+    thus ?case by simp
+  next case (evs_if_f \<Pi> \<sigma> \<phi> \<pi>\<^sub>t \<pi>\<^sub>f \<pi> s \<omega>)
+
+    have "eval_flat_stack (flatten \<Pi>) (state_convert (Bool False # \<sigma>, \<phi>, IfJ \<pi>\<^sub>t \<pi>\<^sub>f # \<pi>, s, \<omega>)) (state_convert (\<sigma>, \<phi>, \<pi>\<^sub>f @ \<pi>, s, \<omega>))" by simp
+    thus ?case by simp
+  next case (evs_call \<Pi> f a l \<Phi> \<sigma> \<phi> \<pi> s \<omega>)
+
+    have "eval_flat_stack (flatten \<Pi>) (state_convert (\<sigma>, \<phi>, Call f # \<pi>, s, \<omega>)) (state_convert ([], Frame f (take a \<sigma>) (repeat (IntV 0) l) (drop a \<sigma>) # \<phi>, \<pi>, s, \<omega>))" by simp
+    thus ?case by simp
+  next case (evs_return \<Pi> \<sigma> f as ls \<phi> \<pi> s \<omega>)
+
+    have "eval_flat_stack (flatten \<Pi>) (state_convert (\<sigma>, Frame f as ls # \<phi>, Return # \<pi>, s, \<omega>)) (state_convert (\<sigma>, \<phi>, \<pi>, s, \<omega>))" by simp
+    thus ?case by simp
+  qed
 
 theorem flattening_correct [simp]: "iterate_ind (eval_stack \<Pi>) \<Sigma> \<Sigma>' \<Longrightarrow>
     iterate_ind (eval_flat_stack (flatten \<Pi>)) (state_convert \<Sigma>) (state_convert \<Sigma>')"
