Stack/StackLanguage.thy
@@ -10,22 +10,31 @@ datatype address =
 datatype stack_instruction = 
   Add | Sub | Neg | Eq | Gt | Lt | And | Or | Not
 | Push address | Pop address
+| IfJ "stack_instruction list" "stack_instruction list" 
+| Goto code_label
+| Call function_name
+| Return
 | Print
 
-type_synonym stack_program = "code_label \<rightharpoonup> stack_instruction list \<times> code_label"
+type_synonym stack_program = 
+  "function_name \<rightharpoonup> nat \<times> nat \<times> (code_label \<rightharpoonup> stack_instruction list \<times> code_label)"
 
 datatype stack_value =
   IntV int
 | Bool bool
 
-datatype frame = Frame "stack_value list" "stack_value list"
+datatype frame = Frame function_name 
+  "stack_value list" (* arguments *)
+  "stack_value list" (* local variables *)
+  "stack_value list" (* saved stack *)
 
 type_synonym stack_state = 
   "stack_value list \<times> frame list \<times> stack_instruction list \<times> code_label \<times> output" 
   (* \<sigma>, \<phi>, \<pi>, s, \<omega> *)
 
 inductive eval_stack :: "stack_program \<Rightarrow> stack_state \<Rightarrow> stack_state \<Rightarrow> bool" where
-  evs_jump [simp]: "\<Pi> s = Some (\<pi>, s') \<Longrightarrow> eval_stack \<Pi> (\<sigma>, \<phi>, [], s, \<omega>) (\<sigma>, \<phi>, \<pi>, s', \<omega>)"
+  evs_jump [simp]: "\<Pi> f = Some (a, l, \<Phi>) \<Longrightarrow> \<Phi> s = Some (\<pi>, s') \<Longrightarrow> 
+    eval_stack \<Pi> (\<sigma>, Frame f as ls \<sigma>' # \<phi>, [], s, \<omega>) (\<sigma>, Frame f as ls \<sigma>' # \<phi>, \<pi>, s', \<omega>)"
 | evs_add [simp]: "eval_stack \<Pi> (IntV i1 # IntV i2 # \<sigma>, \<phi>, Add # \<pi>, s, \<omega>) 
     (IntV (i1 + i2) # \<sigma>, \<phi>, \<pi>, s, \<omega>)"
 | evs_sub [simp]: "eval_stack \<Pi> (IntV i1 # IntV i2 # \<sigma>, \<phi>, Sub # \<pi>, s, \<omega>) 
@@ -43,14 +52,23 @@ inductive eval_stack :: "stack_program \<Rightarrow> stack_state \<Rightarrow> s
     (Bool (i2 \<or> i1) # \<sigma>, \<phi>, \<pi>, s, \<omega>)"
 | evs_not [simp]: "eval_stack \<Pi> (Bool i1 # \<sigma>, \<phi>, Not # \<pi>, s, \<omega>) (Bool (\<not> i1) # \<sigma>, \<phi>, \<pi>, s, \<omega>)"
 | evs_push_c [simp]: "eval_stack \<Pi> (\<sigma>, \<phi>, Push (Constant i) # \<pi>, s, \<omega>) (IntV i # \<sigma>, \<phi>, \<pi>, s, \<omega>)"
-| evs_push_l [simp]: "eval_stack \<Pi> (\<sigma>, Frame as ls # \<phi>, Push (Local n) # \<pi>, s, \<omega>) 
-    (ls ! n # \<sigma>, \<phi>, \<pi>, s, \<omega>)"
-| evs_push_a [simp]: "eval_stack \<Pi> (\<sigma>, Frame as ls # \<phi>, Push (Argument n) # \<pi>, s, \<omega>) 
-    (as ! n # \<sigma>, \<phi>, \<pi>, s, \<omega>)"
-| evs_pop_l [simp]: "eval_stack \<Pi> (v # \<sigma>, Frame as ls # \<phi>, Pop (Local n) # \<pi>, s, \<omega>) 
-    (\<sigma>, Frame as (update_list ls v n) # \<phi>, \<pi>, s, \<omega>)"
-| evs_pop_a [simp]: "eval_stack \<Pi> (v # \<sigma>, Frame as ls # \<phi>, Pop (Argument n) # \<pi>, s, \<omega>) 
-    (\<sigma>, Frame (update_list as v n) ls # \<phi>, \<pi>, s, \<omega>)"
+| evs_push_l [simp]: "eval_stack \<Pi> (\<sigma>, Frame f as ls \<sigma>' # \<phi>, Push (Local n) # \<pi>, s, \<omega>) 
+    (ls ! n # \<sigma>, Frame f as ls \<sigma>' # \<phi>, \<pi>, s, \<omega>)"
+| evs_push_a [simp]: "eval_stack \<Pi> (\<sigma>, Frame f as ls \<sigma>' # \<phi>, Push (Argument n) # \<pi>, s, \<omega>) 
+    (as ! n # \<sigma>, Frame f as ls \<sigma>' # \<phi>, \<pi>, s, \<omega>)"
+| evs_pop_l [simp]: "eval_stack \<Pi> (v # \<sigma>, Frame f as ls \<sigma>' # \<phi>, Pop (Local n) # \<pi>, s, \<omega>) 
+    (\<sigma>, Frame f as (ls[n := v]) \<sigma>' # \<phi>, \<pi>, s, \<omega>)"
+| evs_pop_a [simp]: "eval_stack \<Pi> (v # \<sigma>, Frame f as ls \<sigma>' # \<phi>, Pop (Argument n) # \<pi>, s, \<omega>) 
+    (\<sigma>, Frame f (as[n := v]) ls \<sigma>' # \<phi>, \<pi>, s, \<omega>)"
+| evs_if_t [simp]: "eval_stack \<Pi> (Bool True # \<sigma>, \<phi>, IfJ \<pi>\<^sub>t \<pi>\<^sub>f # \<pi>, s, \<omega>) (\<sigma>, \<phi>, \<pi>\<^sub>t @ \<pi>, s, \<omega>)"
+| evs_if_f [simp]: "eval_stack \<Pi> (Bool False # \<sigma>, \<phi>, IfJ \<pi>\<^sub>t \<pi>\<^sub>f # \<pi>, s, \<omega>) (\<sigma>, \<phi>, \<pi>\<^sub>f @ \<pi>, s, \<omega>)"
+| evs_goto [simp]: "\<Pi> f = Some (a, l, \<Phi>) \<Longrightarrow> \<Phi> s = Some (\<pi>, s') \<Longrightarrow> 
+    eval_stack \<Pi> (\<sigma>, Frame f as ls \<sigma>' # \<phi>, Goto s # \<pi>, s'', \<omega>) (\<sigma>, Frame f as ls \<sigma>' # \<phi>, \<pi>', s', \<omega>)"
+| evs_call [simp]: "\<Pi> f = Some (a, l, \<Phi>) \<Longrightarrow> 
+    eval_stack \<Pi> (\<sigma>, \<phi>, Call f # \<pi>, s, \<omega>) ([], Frame f (take a \<sigma>) 
+      (repeat (IntV 0) l) (drop a \<sigma>) # \<phi>, \<pi>, s, \<omega>)"
+| evs_return [simp]: 
+    "eval_stack \<Pi> (v # \<sigma>, Frame f as ls \<sigma>' # \<phi>, Return # \<pi>, s, \<omega>) (v # \<sigma>', \<phi>, \<pi>, s, \<omega>)"
 | evs_print [simp]: "eval_stack \<Pi> (IntV i1 # \<sigma>, \<phi>, Print # \<pi>, s, \<omega>) (\<sigma>, \<phi>, \<pi>, s, i1 # \<omega>)"
 
 fun stack_output :: "stack_state \<Rightarrow> output" where
